improved HOU compilation time

theories/HOU/concon/constants.v
@@ -1,8 +1,8 @@
-Require Import List Omega Lia Morphisms Setoid.
-From Undecidability.HOU Require Import std.std calculus.calculus.
+Require Import List Arith Lia Morphisms Setoid.
+From Undecidability.HOU Require Import calculus.calculus.
 From Undecidability.HOU Require Import
         unification.higher_order_unification unification.nth_order_unification
-        concon.conservativity.
+        concon.conservativity_constants concon.conservativity.
 Import ListNotations.
 
 Set Default Proof Using "Type".
@@ -327,7 +327,7 @@ Section RemoveConstants.
       all: intros; eapply H0; cbn; simplify; intuition.
   Qed.
 
-  
+
 
   Lemma enc_subst_term_reduce tau s:
     (forall x c, c ∈ consts (tau x) -> R' c = None -> c ∈ C) ->
@@ -525,77 +525,3 @@ Section RemoveConstants.
 
 
 End RemoveConstants.
-
-
-
-(* ** Goldfarb sharp *)
-
-From Undecidability.HOU Require Import
-   second_order.diophantine_equations second_order.goldfarb.reduction.
-
-Definition gonly : Const :=
-  {|
-    const_type := option False;
-    ctype := fun o => match o with
-                  | None => alpha → alpha → alpha
-                  | Some f => match f with end
-                  end
-                    
-  |}.
-
-Program Instance RE_ag_gonly : retract gonly ag :=
-  {|
-    I := fun _ => None;
-    R := fun x => match x with None => Some None | _ => None end
-  |}.
-Next Obligation.
-  now destruct x as [[]|].
-Qed.
-  
-
-
-Lemma Goldfarb_remove:
-  H10 ⪯ OU 2 ag /\ OU 2 ag ⪯ OU 2 gonly.
-Proof.
-  split. eapply Goldfarb.
-  eapply (@remove_constants_reduction ag gonly); eauto.
-  intros [[]|]; cbn; eauto.
-  intros [[[]|]|]; cbn; eauto.
-  destruct eq_dec; intuition  discriminate.
-Qed.
-
-
-Lemma Goldfarb_sharp (C: Const) (re: retract gonly C):
-  ctype C (I None) = alpha → alpha → alpha -> OU 2 gonly ⪯ OU 2 C.
-Proof.
-  intros. eapply unification_constants_monotone; eauto.
-  intros [[]|]; cbn; eauto.
-Qed.
-
-
-Definition cfree : Const :=
-  {|
-    const_type := False;
-    ctype := fun f => match f with end
-  |}.
-
-Program Instance RE_cfree X : retract cfree X :=
-  {|
-    I := fun f => match f with end;
-    R := fun x => None
-  |}.
-
-
-Lemma Goldfarb_Huet X:
-  OU 2 gonly ⪯ OU 3 gonly /\
-  OU 3 gonly ⪯ OU 3 cfree /\
-  OU 3 cfree ⪯ OU 3 X.
-Proof.
-  repeat split. 
-  eapply unification_step; eauto.
-  eapply remove_constants_reduction; eauto.  
-  intros []. intros [[]|]; cbn; eauto.
-  eapply unification_constants_monotone; eauto.
-  intros [].
-Qed.
-         
