theories/HOU/calculus/normalisation.v
@@ -1,6 +1,8 @@
 Set Implicit Arguments.
-Require Import Morphisms Omega Lia. 
-From Undecidability.HOU.calculus Require Export semantics typing order.
+Require Import Morphisms Omega Lia.
+From Undecidability.HOU Require Import std.std.
+From Undecidability.HOU.calculus Require Import 
+  prelim terms syntax semantics confluence typing order. 
 
 Set Default Proof Using "Type".
 
