theories/HOU/calculus/order.v
@@ -1,6 +1,8 @@
 Set Implicit Arguments.
 Require Import List Omega Lia.
-From Undecidability.HOU.calculus Require Export syntax semantics equivalence typing.
+From Undecidability.HOU Require Import std.std.
+From Undecidability.HOU.calculus Require Import 
+  prelim terms syntax semantics typing. 
 
 Set Default Proof Using "Type".
 
