theories/HOU/calculus/semantics.v
@@ -1,5 +1,5 @@
 Set Implicit Arguments.
-From Undecidability.HOU Require Export calculus.syntax std.std.
+From Undecidability.HOU Require Import calculus.prelim calculus.terms calculus.syntax std.std.
 Require Import Morphisms Omega Lia FinFun. 
 
 Set Default Proof Using "Type".
