theories/HOU/calculus/terms_extension.v
@@ -1,8 +1,9 @@
 Set Implicit Arguments.
-Require Import List Omega Lia Morphisms FinFun.
+Require Import List Arith Lia Morphisms FinFun.
 Import ListNotations.
-From Undecidability.HOU.calculus Require Export semantics typing.
-From Undecidability.HOU Require Import calculus.order.
+From Undecidability.HOU Require Import std.std.
+From Undecidability.HOU.calculus Require Import 
+  prelim terms syntax semantics equivalence typing order. 
 
 Set Default Proof Using "Type".
 
@@ -56,13 +57,13 @@ Section TermsExtension.
     Lemma listtyping_app Gamma S1 S2 L1 L2:
       Gamma ⊢₊ S1 : L1 -> Gamma ⊢₊ S2 : L2 -> Gamma ⊢₊ S1 ++ S2 : L1 ++ L2.
     Proof.
-      induction 1; cbn; eauto.  
+      induction 1; cbn; (eauto 3).  
     Qed.
 
     Lemma orderlisttyping_app n Gamma S1 S2 L1 L2:
       Gamma ⊢₊(n) S1 : L1 -> Gamma ⊢₊(n) S2 : L2 -> Gamma ⊢₊(n) S1 ++ S2 : L1 ++ L2.
     Proof.
-      induction 1; cbn; eauto.  
+      induction 1; cbn; (eauto 3).  
     Qed.
 
     Lemma Vars_listtyping x Gamma S L:
@@ -90,7 +91,7 @@ Section TermsExtension.
       (forall s, s ∈ S -> Gamma ⊢(n) s : A) ->
       forall m, m = length S -> Gamma ⊢₊(n) S : repeat A m.
     Proof.
-      induction S; cbn; intros; subst; cbn; eauto.
+      induction S; cbn; intros; subst; cbn; (eauto 2).
       intuition.  
     Qed.
 
@@ -103,13 +104,13 @@ Section TermsExtension.
       - specialize (H a) as H'; mp H'; intuition; domin H'.
         rewrite H' in H0. subst. econstructor.
         all: cbn in H1; simplify in H1; intuition.
-        eapply IHN; eauto; lauto.
+        eapply IHN; (eauto 1); lauto.
     Qed.
 
     Lemma var_typing n Gamma:
       ord' Gamma <= n -> Gamma ⊩(n) @var X : Gamma.
     Proof.
-      intros ????; econstructor; eauto;
+      intros ????; econstructor; (eauto 1);
         eapply ord'_elements; eauto using nth_error_In.
     Qed.
 
@@ -117,36 +118,36 @@ Section TermsExtension.
       ord' (map (ctype X) Cs) <= S n ->
       Gamma ⊢₊(n) map const Cs : map (ctype X) Cs.
     Proof.
-      induction Cs; cbn; eauto.
-      intros H; simplify in H; intuition; econstructor; eauto. 
+      induction Cs; cbn; (eauto 2).
+      intros H; simplify in H; intuition; econstructor; (eauto 2). 
     Qed.
 
 
     Lemma listtyping_preservation_under_renaming delta Gamma Delta S L:
       Gamma ⊢₊ S : L -> Delta ⊫ delta : Gamma -> Delta ⊢₊ renL delta S : L.
     Proof.
-      intros H1 H2; induction H1; cbn; eauto.
+      intros H1 H2; induction H1; cbn; (eauto 3).
     Qed.
 
     Lemma orderlisttyping_preservation_under_renaming n delta Gamma Delta S L:
       Gamma ⊢₊(n) S : L -> Delta ⊫ delta : Gamma -> Delta ⊢₊(n) renL delta S : L.
     Proof.
-      intros H1 H2; induction H1; cbn; eauto.
+      intros H1 H2; induction H1; cbn; (eauto 3).
     Qed.
 
     Lemma orderlisttyping_preservation_under_substitution Gamma n S L Delta sigma:
       Gamma ⊢₊(n) S : L -> Delta ⊩(n) sigma : Gamma -> Delta ⊢₊(n) sigma •₊ S : L.
     Proof.
-      induction 1; cbn; eauto.
+      induction 1; cbn; (eauto 4).
     Qed.
 
     Lemma orderlisttyping_element Gamma n S L:
       Gamma ⊢₊(n) S : L -> forall s, s ∈ S -> exists A, Gamma ⊢(n) s : A /\ A ∈ L.
     Proof.
       induction 1; cbn; intros; intuition; subst.
-      eexists; intuition; eauto.
-      edestruct IHorderlisttyping; eauto; intuition;
-        eexists; split; eauto.
+      eexists; intuition; (eauto 2).
+      edestruct IHorderlisttyping; (eauto 1); intuition;
+        eexists; split; (eauto 2).
     Qed.
 
 
@@ -164,14 +165,14 @@ Section TermsExtension.
     Lemma list_equiv_ren delta S T:
       S ≡₊ T -> renL delta S ≡₊ renL delta T.
     Proof.
-      intros; pattern S, T; eapply list_equiv_ind; eauto.
+      intros; pattern S, T; eapply list_equiv_ind; (eauto 2).
       intros s t S' T' H1 H2 IH; cbn; now rewrite H1, IH. 
     Qed.
 
     Lemma list_equiv_subst sigma S T:
       S ≡₊ T -> (sigma •₊ S) ≡₊ (sigma •₊ T).
     Proof.
-      intros; pattern S, T; eapply list_equiv_ind; eauto.
+      intros; pattern S, T; eapply list_equiv_ind; (eauto 2).
       intros s t S' T' H1 H2 IH; cbn; now rewrite H1, IH.
     Qed.
 
@@ -181,13 +182,13 @@ Section TermsExtension.
     Proof.
       intros In. remember (renL delta S) as S'. remember (renL delta T) as T'.
       intros H; revert S T HeqS' HeqT'; pattern S', T'. 
-      eapply list_equiv_ind; eauto.
+      eapply list_equiv_ind; (eauto 2).
       all: intros. 
       - destruct S, T; try discriminate. reflexivity.
       - destruct S0, T0; try discriminate.
         injection HeqS' as ??; injection HeqT' as ??; subst.
-        eapply equiv_lstep_cons_proper; eauto.
-        eapply equiv_anti_ren; eauto.
+        eapply equiv_lstep_cons_proper; (eauto 2).
+        eapply equiv_anti_ren; (eauto 2).
     Qed.
 
     Global Instance list_ren_proper delta:
@@ -236,8 +237,8 @@ Section TermsExtension.
       - intros _. exists L2. intuition.
       - destruct L2. inversion 1.
         intros H H1. cbn in H. eapply le_S_n in H.
-        injection H1 as ??. subst. edestruct IHL1; eauto.
-        intuition. exists x; intuition. f_equal; eauto.
+        injection H1 as ??. subst. edestruct IHL1; (eauto 2).
+        intuition. exists x; intuition. f_equal; (eauto 2).
     Qed.
 
 
@@ -266,8 +267,8 @@ Section TermsExtension.
       Arr L1 A = Arr L2 A -> L1 = L2.
     Proof.
       destruct (le_ge_dec (length L1) (length L2)); intros H; [|symmetry in H].
-      all: eapply Arr_inversion in H as [L3]; eauto; intuition.
-      all: destruct L3; simplify in *; eauto.
+      all: eapply Arr_inversion in H as [L3]; (eauto 1); intuition.
+      all: destruct L3; simplify in *; (eauto 2).
       all: eapply (f_equal arity) in H1; cbn in H1; rewrite arity_Arr in H1.
       all: lia.
     Qed.
@@ -288,7 +289,7 @@ Section TermsExtension.
 
     Lemma ord_repeated n A: ord' (repeat A n) <= ord A.
     Proof.
-      induction n; cbn; eauto.
+      induction n; cbn; (eauto 2).
       lia. 
     Qed.
 
@@ -354,7 +355,7 @@ Section TermsExtension.
   
   Lemma AppR_head s T: head (AppR s T) = head s.
   Proof.
-    induction T in s |-*; cbn ; eauto; now rewrite IHA. 
+    induction T in s |-*; cbn ; (eauto 1); now rewrite IHA. 
   Qed.
 
   Hint Rewrite AppR_head : simplify.
@@ -367,7 +368,7 @@ Section TermsExtension.
     Lemma Lambda_ren delta n s:
       ren delta (Lambda n s) = Lambda n (ren (it n up_ren delta) s).
     Proof.
-      induction n in delta |-*; cbn; eauto.
+      induction n in delta |-*; cbn; (eauto 2).
       rewrite IHn. do 3 f_equal. 
       symmetry. eapply it_commute.
     Qed.
@@ -375,7 +376,7 @@ Section TermsExtension.
     Lemma Lambda_subst sigma n s:
       sigma • (Lambda n s) = Lambda n (it n up sigma • s).
     Proof.
-      induction n in sigma |-*; cbn; eauto.
+      induction n in sigma |-*; cbn; (eauto 2).
       rewrite IHn; do 3 f_equal.
       symmetry. eapply it_commute.
     Qed.
@@ -416,50 +417,50 @@ Section TermsExtension.
     Global Instance Lambda_step_proper k:
       Proper (step ++> step) (Lambda k).
     Proof.
-      induction k; cbn; intros ??; eauto.
+      induction k; cbn; intros ??; (eauto 3).
     Qed.
 
     Global Instance AppR_step_proper:
       Proper (step ++> eq ++> step) AppR.
     Proof.
       intros s t ? ? A ->.
-      induction A in s, t, H |-*; cbn; eauto.
+      induction A in s, t, H |-*; cbn; (eauto 3).
     Qed.
 
     Global Instance AppR_lstep_proper:
       Proper (eq ++> lstep step ++> step) AppR.
     Proof.
       intros ? ? -> ? ? H.
-      induction H in y |-*; cbn; eauto.
+      induction H in y |-*; cbn; (eauto 2).
     Qed. 
 
     Global Instance AppL_step_proper:
       Proper (eq ++> step ++> step) AppL.
     Proof.
       intros ? A -> s t H.
-      induction A in s, t, H |-*; cbn; eauto.
+      induction A in s, t, H |-*; cbn; (eauto 3).
     Qed.
 
     Global Instance AppL_lstep_proper:
       Proper (lstep step ++> eq ++> step) AppL.
     Proof.
       intros ? ? H ? t ->.
-      induction H in t |-*; cbn; eauto.
+      induction H in t |-*; cbn; (eauto 2).
     Qed. 
 
     Global Instance Lambda_steps_proper k:
       Proper (star step ++> star step) (Lambda k).
     Proof.
-      induction 1; eauto; now rewrite H.
+      induction 1; (eauto 1); now rewrite H.
     Qed.
 
     Global Instance AppL_proper:
       Proper (star (lstep step) ++> star step ++> star step) AppL.
     Proof.
       intros ? ?. induction 1.
-      - intros ? ? ?. induction H; cbn; eauto. 
+      - intros ? ? ?. induction H; cbn; (eauto 2). 
         rewrite <-IHstar. 
-        econstructor 2; eauto; eapply AppL_step_proper; eauto.
+        econstructor 2; (eauto 1); eapply AppL_step_proper; (eauto 2).
       - intros ? ? ?. rewrite H. specialize (IHstar _ _ H1).
         now rewrite IHstar. 
     Qed.
@@ -468,9 +469,9 @@ Section TermsExtension.
       Proper (star step ++> star (lstep step) ++> star step) AppR.
     Proof.
       intros ? ?. induction 1.
-      - intros ? ? ?. induction H; cbn; eauto. 
+      - intros ? ? ?. induction H; cbn; (eauto 2). 
         rewrite <-IHstar.
-        econstructor 2; eauto; eapply AppR_lstep_proper; eauto.
+        econstructor 2; (eauto 1); eapply AppR_lstep_proper; (eauto 2).
       - intros ? ? ?. rewrite H. specialize (IHstar _ _ H1).
         now rewrite IHstar. 
     Qed.
@@ -478,7 +479,7 @@ Section TermsExtension.
     Global Instance Lambda_equiv_proper n:
       Proper (equiv step ++> equiv step) (Lambda n).
     Proof.
-      intros ? ? ?; induction n; cbn; eauto.
+      intros ? ? ?; induction n; cbn; (eauto 2).
       now rewrite IHn. 
     Qed.
 
@@ -493,7 +494,7 @@ Section TermsExtension.
     Global Instance equiv_AppR_proper:
       Proper (equiv step ++> equiv (lstep step) ++> equiv step) AppR.
     Proof.
-      intros ? ? (? & H1 & H2) % church_rosser ? ? (? & H3 & H4) % church_rosser; eauto.
+      intros ? ? (? & H1 & H2) % church_rosser ? ? (? & H3 & H4) % church_rosser; (eauto 2).
       now rewrite H1, H2, H3, H4. 
     Qed.  
 
@@ -504,9 +505,9 @@ Section TermsExtension.
   Lemma AppR_Lambda T s n sigma:
     AppR (sigma • Lambda (length T + n) s) T >* T .+ sigma • Lambda n s.
   Proof.
-    revert s n sigma; induction T; intros; cbn [AppR length]; eauto. 
+    revert s n sigma; induction T; intros; cbn [AppR length]; (eauto 2). 
     replace (S (length T) + n) with (length T + S n) by lia.
-    rewrite IHT; cbn; econstructor 2; eauto; now asimpl. 
+    rewrite IHT; cbn; econstructor 2; (eauto 2); now asimpl. 
   Qed.
 
   Lemma AppR_Lambda' T s m:
@@ -533,8 +534,8 @@ Section TermsExtension.
       isAtom s2 ->
       T1 ≡₊ T2 /\ s1 = s2.
     Proof.
-      intros; assert (isAtom (head (AppR s1 T1))); simplify; eauto.
-      intros; assert (isAtom (head (AppR s2 T2))); simplify; eauto.
+      intros; assert (isAtom (head (AppR s1 T1))); simplify; (eauto 2).
+      intros; assert (isAtom (head (AppR s2 T2))); simplify; (eauto 2).
       
       revert T2 H H2 H3; induction T1 as [|a A IH]; intros [| b B]; cbn; intros.
       + intuition.
@@ -542,7 +543,7 @@ Section TermsExtension.
         all: Injection H; now subst. 
       + destruct s1; cbn in *; try now intuition; Discriminate.
       + destruct s2; cbn in *; try now intuition; Discriminate. 
-      + Injection H. intuition; edestruct IH; eauto.
+      + Injection H. intuition; edestruct IH; (eauto 2).
         now rewrite H5, H. 
     Qed.
 
@@ -557,8 +558,8 @@ Section TermsExtension.
         cbn; intros;
         try discriminate.
       + intuition. 
-      + apply equiv_app_elim in H as ?; rewrite ?AppR_head; eauto.
-        intuition; edestruct IH; eauto.
+      + apply equiv_app_elim in H as ?; rewrite ?AppR_head; (eauto 3).
+        intuition; edestruct IH; (eauto 3).
         now rewrite H3, H4.
     Qed.
 
@@ -579,7 +580,7 @@ Section TermsExtension.
       normal (AppL S t) -> Normal (lstep step) S.
     Proof.
       induction S; cbn; intros H ? H1; inv H1.
-      - eapply H; eauto.
+      - eapply H; (eauto 2).
       - eapply IHS; eauto using normal_app_r.
     Qed.
 
@@ -619,11 +620,11 @@ Section TermsExtension.
     Proof.
       induction k in L, Gamma, s |-*.
       - destruct L; try discriminate.
-        intros _; cbn; eauto.
+        intros _; cbn; (eauto 2).
       - destruct L; try discriminate.
         intros H; injection H as H.
         cbn; intros; econstructor.
-        eapply IHk; eauto.
+        eapply IHk; (eauto 2).
         now rewrite <-app_assoc in H0. 
     Qed.
 
@@ -634,11 +635,11 @@ Section TermsExtension.
     Proof.
       induction k in L, Gamma, s |-*.
       - destruct L; try discriminate.
-        intros _; cbn; eauto.
+        intros _; cbn; (eauto 2).
       - destruct L; try discriminate.
         intros H; injection H as H.
         cbn; intros; econstructor.
-        eapply IHk; eauto.
+        eapply IHk; (eauto 2).
         now rewrite <-app_assoc in H0.
     Qed.
 
@@ -646,22 +647,22 @@ Section TermsExtension.
     Lemma AppL_typing_repeated Gamma s T n A:
       Gamma ⊢₊ T: repeat (A → A) n -> Gamma ⊢ s : A -> Gamma ⊢ AppL T s : A.
     Proof.
-      induction T in n |-*; eauto; cbn.
+      induction T in n |-*; (eauto 1); cbn.
       intros; inv H; intuition.
       destruct n; try discriminate.
       cbn in H3; injection H3 as ??; subst.  
-      econstructor; eauto. 
+      econstructor; (eauto 2). 
     Qed.
 
 
     Lemma AppL_ordertyping_repeated k Gamma s T n A:
       Gamma ⊢₊(n) T: repeat (A → A) k -> Gamma ⊢(n) s : A -> Gamma ⊢(n) AppL T s : A.
     Proof.
-      induction T in k |-*; eauto; cbn.
+      induction T in k |-*; (eauto 1); cbn.
       intros; inv H; intuition.
       destruct k; try discriminate.
       cbn in H3; injection H3 as ??; subst.  
-      econstructor; eauto.
+      econstructor; (eauto 2).
     Qed.
 
 
@@ -669,13 +670,13 @@ Section TermsExtension.
     Lemma AppR_typing Gamma L s T B:
       Gamma ⊢₊ T : L -> Gamma ⊢ s : Arr (rev L) B -> Gamma ⊢ AppR s T : B.
     Proof.
-      induction 1 in s, B |-*; cbn; eauto; rewrite Arr_app; cbn; eauto.  
+      induction 1 in s, B |-*; cbn; (eauto 1); rewrite Arr_app; cbn; (eauto 3).  
     Qed.
 
     Lemma AppR_ordertyping n Gamma T s L B:
       Gamma ⊢₊(n) T : L -> Gamma ⊢(n) s : Arr (rev L) B -> Gamma ⊢(n) AppR s T : B.
     Proof.
-      induction 1 in s, B |-*; cbn; eauto; rewrite Arr_app; cbn; eauto.  
+      induction 1 in s, B |-*; cbn; (eauto 1); rewrite Arr_app; cbn; (eauto 3).  
     Qed.
 
     Lemma Lambda_typing_inv Gamma s k B:
@@ -686,7 +687,7 @@ Section TermsExtension.
       induction k in Gamma, B |-*; cbn.
       - exists nil. exists B. intuition.
       - intros H; inv H.
-        edestruct IHk as (? & ? & ?); eauto.
+        edestruct IHk as (? & ? & ?); (eauto 2).
         intuition. exists (A :: x). exists x0.
         intuition; cbn; try congruence.
         now rewrite <-app_assoc.
@@ -700,7 +701,7 @@ Section TermsExtension.
       induction k in Gamma, B |-*; cbn.
       - exists nil. exists B. cbn in *; intuition.
       - intros H; inv H.
-        edestruct IHk as (? & ? & ?); eauto.
+        edestruct IHk as (? & ? & ?); (eauto 2).
         intuition. exists (A :: x). exists x0.
         intuition; cbn; try congruence.
         now rewrite <-app_assoc.
@@ -713,8 +714,8 @@ Section TermsExtension.
       induction T in B |-*; cbn.
       - exists nil. exists B. intuition.
       - intros H; inv H.
-        edestruct IHT as (? & ? & ?); eauto.
-        do 2 eexists; intuition; eauto.
+        edestruct IHT as (? & ? & ?); (eauto 2).
+        do 2 eexists; intuition; (eauto 2).
     Qed.
 
     Lemma AppL_ordertyping_inv n Gamma T B t:
@@ -723,8 +724,8 @@ Section TermsExtension.
       induction T in B |-*; cbn.
       - exists nil. exists B. intuition.
       - intros H; inv H.
-        edestruct IHT as (? & ? & ?); eauto.
-        do 2 eexists; intuition; eauto.
+        edestruct IHT as (? & ? & ?); (eauto 2).
+        do 2 eexists; intuition; (eauto 2).
     Qed.
 
     Lemma AppR_typing_inv Gamma T B t:
@@ -733,7 +734,7 @@ Section TermsExtension.
       induction T in Gamma, B, t |-*; cbn; intros.
       - exists nil; intuition.
       - inv H. destruct (IHT _ _ _ H2) as [L]; intuition.
-        exists (A :: L). intuition; cbn; rewrite Arr_app; eauto. 
+        exists (A :: L). intuition; cbn; rewrite Arr_app; (eauto 2). 
     Qed.
 
 
@@ -743,7 +744,7 @@ Section TermsExtension.
       induction T in Gamma, B, t |-*; cbn; intros.
       - exists nil; intuition.
       - inv H. destruct (IHT _ _ _ H2) as [L]; intuition.
-        exists (A :: L). intuition; cbn; rewrite Arr_app; eauto. 
+        exists (A :: L). intuition; cbn; rewrite Arr_app; (eauto 2). 
     Qed.
 
   End ListOperatorsTyping.
@@ -767,13 +768,13 @@ Section TermsExtension.
       + intros. exists 0 (const c) nil; cbn; intuition.
       + intros H; mp IHs; eauto using normal_lam_elim;
           destruct IHs as [k s' t' T H1].
-        exists (S k) s' T; eauto; cbn; congruence.
+        exists (S k) s' T; (eauto 1); cbn; congruence.
       + intros H; eapply normal_app_r in H as Ns1;
         eapply normal_app_l in H as Ns2.  
-        mp IHs1; eauto; mp IHs2; eauto.
+        mp IHs1; (eauto 1); mp IHs2; (eauto 2).
         destruct IHs1. subst t.
         destruct k; [|exfalso; eapply H; cbn; eauto].
-        exists 0 s (s2 :: T); eauto; cbn; simplify.
+        exists 0 s (s2 :: T); (eauto 1); cbn; simplify.
         intros t. destruct (s2 == t); subst; intuition.
         destruct (t el T); intuition.
         exfalso; intuition.
@@ -792,7 +793,7 @@ Section TermsExtension.
       - exists nil. exists (lambda s). cbn; intuition; discriminate.
       - destruct IHs2 as (S & t & ? & -> & ?).
         destruct (D s1).
-        + exists (s1 :: S). exists t; cbn; intuition; subst; eauto.
+        + exists (s1 :: S). exists t; cbn; intuition; subst; (eauto 2).
         + exists nil. exists (s1 (AppL S t)). cbn; intuition.
           injection H1 as ??;subst; intuition.
     Qed.
