theories/HOU/concon/constants_consequences.v
@@ -1,0 +1,77 @@
+Require Import List Arith Lia Morphisms Setoid.
+From Undecidability.HOU Require Import calculus.calculus.
+From Undecidability.HOU Require Import
+        unification.higher_order_unification unification.nth_order_unification
+        concon.conservativity_constants concon.conservativity concon.constants.
+Import ListNotations.
+
+(* ** Goldfarb sharp *)
+
+From Undecidability.HOU Require Import
+   second_order.diophantine_equations second_order.goldfarb.reduction.
+
+Definition gonly : Const :=
+  {|
+    const_type := option False;
+    ctype := fun o => match o with
+                  | None => alpha → alpha → alpha
+                  | Some f => match f with end
+                  end
+                    
+  |}.
+
+Program Instance RE_ag_gonly : retract gonly ag :=
+  {|
+    I := fun _ => None;
+    R := fun x => match x with None => Some None | _ => None end
+  |}.
+Next Obligation.
+  now destruct x as [[]|].
+Qed.
+  
+
+
+Lemma Goldfarb_remove:
+  H10 ⪯ OU 2 ag /\ OU 2 ag ⪯ OU 2 gonly.
+Proof.
+  split. eapply Goldfarb.
+  eapply (@remove_constants_reduction ag gonly); eauto.
+  intros [[]|]; cbn; eauto.
+  intros [[[]|]|]; cbn; eauto.
+  destruct eq_dec; intuition  discriminate.
+Qed.
+
+
+Lemma Goldfarb_sharp (C: Const) (re: retract gonly C):
+  ctype C (I None) = alpha → alpha → alpha -> OU 2 gonly ⪯ OU 2 C.
+Proof.
+  intros. eapply unification_constants_monotone; eauto.
+  intros [[]|]; cbn; eauto.
+Qed.
+
+
+Definition cfree : Const :=
+  {|
+    const_type := False;
+    ctype := fun f => match f with end
+  |}.
+
+Program Instance RE_cfree X : retract cfree X :=
+  {|
+    I := fun f => match f with end;
+    R := fun x => None
+  |}.
+
+
+Lemma Goldfarb_Huet X:
+  OU 2 gonly ⪯ OU 3 gonly /\
+  OU 3 gonly ⪯ OU 3 cfree /\
+  OU 3 cfree ⪯ OU 3 X.
+Proof.
+  repeat split. 
+  eapply unification_step; eauto.
+  eapply remove_constants_reduction; eauto.  
+  intros []. intros [[]|]; cbn; eauto.
+  eapply unification_constants_monotone; eauto.
+  intros [].
+Qed.
