theories/HOU/second_order/diophantine_equations.v
@@ -1,5 +1,5 @@
 Require Import Omega Lia List.
-From Undecidability.HOU Require Import calculus.prelim.
+From Undecidability.HOU Require Import std.std calculus.prelim.
 Import ListNotations.
 
 (* * H10 *)
