theories/HOU/second_order/goldfarb/multiplication.v
@@ -2,7 +2,7 @@ Set Implicit Arguments.
 Require Import List Lia Program.Program.
 From Undecidability.HOU Require Import std.std axioms.
 Require Import RelationClasses Morphisms Wf Init.Nat Setoid.
-From Undecidability.HOU Require Import calculus.calculus unification.unification second_order.goldfarb.encoding.
+From Undecidability.HOU Require Import calculus.calculus second_order.goldfarb.encoding.
 Require Import FinFun Coq.Arith.Wf_nat.
 Import ListNotations.
 
