theories/HOU/third_order/huet.v
@@ -22,25 +22,25 @@ Section HuetReduction.
     (lambda lambda lambda h (AppR f (Enc 1 2 (heads S))) (AppR f (repeat (var (u 1)) (length S)))) :
     ((alpha → alpha) → (alpha → alpha) → (alpha → alpha → alpha) →  alpha).
   Proof.
-    do 4 econstructor. econstructor. econstructor; cbn; eauto; cbn; eauto.
+    do 4 econstructor. econstructor. econstructor; cbn; (eauto 1); cbn; (eauto 2).
     - eapply AppR_ordertyping with (L := repeat (alpha → alpha)  (length S) ); simplify.
       erewrite <-map_length; eapply Enc_typing.
-      all: econstructor; eauto.
-      simplify; cbn; eauto. 
+      all: econstructor; (eauto 2).
+      simplify; cbn; (eauto 3). 
     - eapply AppR_ordertyping. 
       + eapply repeated_ordertyping; simplify; [|eauto]. 
         intros s H'. eapply repeated_in in H'. subst.
         econstructor; cbn. 2: eauto. eauto.
-      + econstructor; simplify; eauto.
+      + econstructor; simplify; (eauto 3).
   Qed.
 
   Lemma HGamma₀t₀A₀ (S: list card) : 
     [Arr (repeat (alpha → alpha) (length S)) alpha; (alpha → alpha) → alpha] ⊢( 3) 
     (lambda lambda lambda h (AppR f (Enc 1 2 (tails S))) (var (u 1) (g (var (u 1))))) :
     ((alpha → alpha) → (alpha → alpha) → (alpha → alpha → alpha) →  alpha).
-  Proof with cbn [ord' ord alpha]; simplify; cbn; eauto.
-    do 4 econstructor. econstructor. econstructor; eauto...
-    cbn; eauto. 
+  Proof with cbn [ord' ord alpha]; simplify; cbn; (eauto 3).
+    do 4 econstructor. econstructor. econstructor; (eauto 2)...
+    cbn; (eauto 4). 
     2: do 2 econstructor...
     2 - 3: econstructor...
     eapply AppR_ordertyping with (L := repeat (alpha → alpha) (length S)); simplify.
@@ -50,7 +50,7 @@ Section HuetReduction.
 
   (* ** Reduction Function *)
   Instance PCP_to_U (S: list card) : orduni 3 X.
-  Proof with cbn [ord' ord alpha]; simplify; cbn; eauto.
+  Proof with cbn [ord' ord alpha]; simplify; cbn; (eauto 2).
     refine {|
       Gamma₀ := [Arr (repeat (alpha → alpha) (length S)) alpha; (alpha → alpha) → alpha];
       s₀ :=  lambda lambda lambda h (AppR f (Enc 1 2 (heads S))) (AppR f (repeat (var (u 1)) (length S)));
@@ -73,9 +73,9 @@ Section HuetReduction.
     Proof.
       econstructor. eapply AppL_ordertyping_repeated.
       eapply repeated_ordertyping.
-      intros ? ? % repeated_in; subst; eauto.
-      simplify; eauto.
-      econstructor; eauto.
+      intros ? ? % repeated_in; subst; (eauto 2).
+      simplify; (eauto 2).
+      econstructor; (eauto 2).
     Qed.
 
     Lemma ginst_equivalence I (S: stack):
@@ -86,14 +86,14 @@ Section HuetReduction.
       intros H H0. unfold finst. rewrite !Lambda_ren, !AppL_ren.
       rewrite !map_id_list.
       2: intros ? ?; mapinj; cbn; eapply H0, nats_lt in H3; now rewrite it_up_ren_lt.
-      rewrite AppR_Lambda'; simplify; eauto.
+      rewrite AppR_Lambda'; simplify; (eauto 2).
       unfold ginst; cbn [ren]; erewrite stepBeta.
-      2: asimpl; simplify; cbn; unfold funcomp; eauto.      
-      cbn [ren]. rewrite it_up_ren_ge; simplify; eauto.
-      asimpl. rewrite select_variables_subst; simplify; eauto.
-      rewrite select_repeated; eauto.
+      2: asimpl; simplify; cbn; unfold funcomp; (eauto 2).      
+      cbn [ren]. rewrite it_up_ren_ge; simplify; (eauto 2).
+      asimpl. rewrite select_variables_subst; simplify; (eauto 2).
+      rewrite select_repeated; (eauto 2).
       unfold ginst; cbn; asimpl; simplify.
-      rewrite sapp_ge_in; simplify; eauto.
+      rewrite sapp_ge_in; simplify; (eauto 3).
       replace (_ - _) with 3 by lia.
       destruct I; intuition.
     Qed.
@@ -108,13 +108,13 @@ Section HuetReduction.
       - intros x A. destruct x as [| [| x]]; try discriminate; cbn.
         3: intros [] % nth_error_In. 
         all: injection 1 as ?; subst.
-        eapply finst_typing; eauto.
+        eapply finst_typing; (eauto 2).
         eapply ginst_typing.
       - cbn -[ginst].  do 3 eapply equiv_lam_proper.
         eapply equiv_app_proper.
         eapply equiv_app_proper. reflexivity.
         all: unfold shift, var_zero.
-        all: rewrite !AppR_subst; rewrite ?Enc_subst_id; eauto.        
+        all: rewrite !AppR_subst; rewrite ?Enc_subst_id; (eauto 2).        
         2: rewrite map_id_list.
         3: intros ? ? % repeated_in; subst; reflexivity.
         all: cbn; rewrite !ren_plus_base, !ren_plus_combine;
@@ -123,8 +123,8 @@ Section HuetReduction.
         2: unfold up_ren, funcomp; cbn [scons].
         replace (|S|) with (|heads S|) at 1 by now simplify.
         replace (|S|) with (|tails S|) at 1 by now simplify.
-        rewrite !finst_equivalence, H1; simplify; eauto. 
-        rewrite ginst_equivalence; eauto. 
+        rewrite !finst_equivalence, H1; simplify; (eauto 2). 
+        rewrite ginst_equivalence; (eauto 2). 
         unfold ginst; asimpl. now simplify.  
     Qed.
 
@@ -140,7 +140,7 @@ Section HuetReduction.
     Lemma end_is_var:
       (forall x, x ∈ S -> isVar x) -> exists i e, i < |S| /\ s = var i e.
     Proof using x t sigma N H1 EQ.
-      intros H2; edestruct @end_head_var with (X:=X) as (h' & T & s' & H5 & ?); eauto. subst s. 
+      intros H2; edestruct @end_head_var with (X:=X) as (h' & T & s' & H5 & ?); (eauto 2). subst s. 
       destruct T as [| t1 [| t2 T]]. 
       all: cbn in EQ; specialize (H1 h'). 
       all: destruct (sigma h') eqn: H'; cbn in *; intuition.
@@ -148,11 +148,11 @@ Section HuetReduction.
       1, 2: eapply nth_error_sapp in H; rewrite ?H in EQ.
       + destruct s'; cbn in *; intuition.  Discriminate.
       + rewrite AppR_subst in EQ; cbn in EQ. 
-        eapply equiv_app_elim in EQ as (EQ1 & EQ2); cbn; eauto; simplify.
+        eapply equiv_app_elim in EQ as (EQ1 & EQ2); cbn; (eauto 1); simplify.
         destruct s'; cbn in *; intuition.
-        rewrite H in EQ1. 2: rewrite H; eauto.
+        rewrite H in EQ1. 2: rewrite H; (eauto 3).
         exfalso. symmetry in EQ1.
-        eapply equiv_neq_var_app; eauto; simplify; eauto.  
+        eapply equiv_neq_var_app; (eauto 1); simplify; (eauto 3).  
       + exists h'. exists t1. intuition. eauto using nth_error_Some_lt.
       Unshelve. exact 0.
     Qed.
@@ -184,7 +184,7 @@ Section HuetReduction.
     assert (|L | <= |S'|) as L1 by
           (eapply (f_equal arity) in H1; simplify in H1; rewrite H1; eauto).
     symmetry in H1; eapply Arr_inversion in H1 as (L2 & H1 & H2); simplify; try lia.
-    eapply repeated_app_inv in H1 as (H1 & H3 & H4); eauto.
+    eapply repeated_app_inv in H1 as (H1 & H3 & H4); (eauto 2).
     rewrite H4 in H2; subst B.
     rewrite H3 in *; simplify in *. clear H3 H4 L1. revert H0 H1 EQ1 EQ2 T2 N2.
     generalize (length L); generalize (length L2); clear L L2. intros l k H0 H1 EQ1 EQ2 T2 N2.
@@ -192,8 +192,8 @@ Section HuetReduction.
     rewrite !Lambda_ren in EQ1; rewrite !Lambda_ren in EQ2. 
     simplify in EQ1 EQ2; rewrite !AppR_app in EQ1; rewrite !AppR_app in EQ2.
     simplify in H1; assert (length S1 = l) as H2 by lia; clear H1; subst.
-    rewrite !AppR_Lambda' in EQ1, EQ2; simplify; eauto.
-    rewrite AppR_Lambda' in EQ2; simplify; eauto.
+    rewrite !AppR_Lambda' in EQ1, EQ2; simplify; (eauto 2).
+    rewrite AppR_Lambda' in EQ2; simplify; (eauto 2).
     rewrite it_up_var_sapp in EQ1; simplify; intros; try lia.
     rewrite !it_up_var_sapp in EQ2; simplify; intros; try lia. 
 
@@ -204,41 +204,41 @@ Section HuetReduction.
       rewrite !AppL_subst in EQ1; rewrite !AppL_subst in EQ2. cbn -[add] in *.
       rewrite !select_variables_subst in EQ2. 
       rewrite !select_variables_subst in EQ1.
-      all: simplify; eauto. 
+      all: simplify; (eauto 2). 
       rewrite <-!select_map, !enc_concat in EQ2.
       eapply AppL_ordertyping_inv in T2 as (L' & B & H8 & H9).
-      eapply enc_eq in EQ2; eauto.
+      eapply enc_eq in EQ2; (eauto 2).
       2 - 3: split; intros EQ3;
         eapply end_is_var_typed in EQ3 as (? & ? & ? & ?); cbn; simplify.
       6, 9, 15, 21 :now eauto. 
       3, 8, 13, 16 : now eauto.
       (* close False goals *) 
-      2, 6, 10, 13: eapply H3; cbn; eauto; cbn; now simplify in *.
+      2, 6, 10, 13: eapply H3; cbn; (eauto 1); cbn; now simplify in *.
       (* close normal term goals *)
       3, 5, 8, 11: eauto.
       (* close typing goals *)
       3, 5, 9: eauto. 3, 4, 6:eauto.
       (* close var goals *)
       2 - 3: intros; cbn; unfold funcomp, u, v; intuition discriminate.
-      exists I; intuition; eauto using nats_lt; eauto.
-      2: rewrite <-!select_map; eauto. 
+      exists I; intuition; eauto using nats_lt; (eauto 2).
+      2: rewrite <-!select_map; (eauto 2). 
       subst; cbn [map select concat AppL] in H6, EQ1.
       eapply end_is_var in EQ1 as (? & ? & ? & ?);
         eauto; simplify.
-      eapply H3; cbn; eauto; cbn; now simplify in *.
+      eapply H3; cbn; (eauto 1); cbn; now simplify in *.
       intros; cbn; intuition; discriminate.
-      intros ? ? % repeated_in; subst; eauto.
+      intros ? ? % repeated_in; subst; (eauto 2).
     + eapply id in T2 as T3. 
       eapply AppR_ordertyping_inv in T2 as (L' & T2 & T4).          
-      destruct x as [i | | |]; cbn in H; eauto.  
+      destruct x as [i | | |]; cbn in H; (eauto 2).  
       * inv T4.       
         assert (i < length S2 \/ i >= length S2) as [H42|H42] by lia.
-        ** rewrite nth_error_app1, nth_error_repeated in H6; simplify; eauto.
+        ** rewrite nth_error_app1, nth_error_repeated in H6; simplify; (eauto 2).
            injection H6 as H6. eapply (f_equal ord) in H6. simplify in H6.
            symmetry in H6; eapply Nat.eq_le_incl in H6; simplify in H6.
            intuition. cbn in H6. lia. 
-        ** rewrite <-H2 in EQ1. asimpl in EQ1. rewrite sapp_ge_in in EQ1; simplify; eauto.
-           eapply equiv_head_equal in EQ1; simplify; cbn; eauto.
+        ** rewrite <-H2 in EQ1. asimpl in EQ1. rewrite sapp_ge_in in EQ1; simplify; (eauto 2).
+           eapply equiv_head_equal in EQ1; simplify; cbn; (eauto 2).
            simplify in EQ1; cbn in EQ1. discriminate EQ1.
       * rewrite <-H2 in EQ1. exfalso. asimpl in EQ1. 
         eapply equiv_head_equal in EQ1; cbn; simplify; cbn; intuition.
